start using separation logic to define containsProgram

compiler/src/GoFlatToRiscv.v
@@ -1,6 +1,6 @@
 Require Import Coq.ZArith.BinInt.
 Require Import Coq.Lists.List. Import ListNotations.
-Require Import coqutil.Map.Interface.
+Require Import coqutil.Map.Interface coqutil.Map.Properties.
 Require Import coqutil.Word.Interface coqutil.Word.Properties.
 Require Import riscv.util.Monads.
 Require Import riscv.Utility.
@@ -15,6 +15,8 @@ Require Import coqutil.Tactics.Tactics.
 Require Import compiler.containsProgram.
 Require Import compiler.FlatToRiscvBitWidthSpecifics.
 Require Import compiler.util.Tactics.
+Require Import compiler.SeparationLogic.
+
 
 Local Unset Universe Polymorphism.
 
@@ -24,6 +26,7 @@ Section Go.
   Context {RFF: RegisterFileFunctions Register word}.
   Context {Action: Type}.
   Context {mem: map.map word byte}.
+  Context {mem_ok: map.ok mem}.
 
   Local Notation RiscvMachineL := (RiscvMachine Register Action).
 
@@ -63,26 +66,89 @@ Section Go.
     intros. rewrite associativity. assumption.
   Qed.
 
-  Lemma go_fetch_inst: forall {inst initialL pc0} (post: RiscvMachineL -> Prop),
+  Fixpoint ptsto_bytes(n: nat)(addr: word): HList.tuple byte n -> mem -> Prop :=
+    match n with
+    | O => fun _ => emp True
+    | S n0 => fun bytes =>
+                sep (ptsto addr (PrimitivePair.pair._1 bytes))
+                    (ptsto_bytes n0 (word.add addr (word.of_Z 1)) (PrimitivePair.pair._2 bytes))
+    end.
+
+  Lemma impl1_sep_cancel_l: forall P Q1 Q2,
+      impl1 Q1 Q2 -> impl1 (P * Q1)%type (P * Q2)%type.
+  Proof.
+    unfold impl1 in *.
+    intros.
+    unfold sep in *.
+    destruct_products.
+    eauto 10.
+  Qed.
+
+  Lemma impl1_sep_cancel_r: forall P Q1 Q2,
+      impl1 Q1 Q2 -> impl1 (Q1 * P)%type (Q2 * P)%type.
+  Proof.
+    unfold impl1 in *.
+    intros.
+    unfold sep in *.
+    destruct_products.
+    eauto 10.
+  Qed.
+
+  Lemma ptsto_bytes_to_load: forall n m v addr R,
+      (ptsto_bytes n addr v * R)%type m ->
+      Memory.load n m addr = Some v.
+  Proof.
+    induction n; intros.
+    - simpl in *. destruct v. reflexivity.
+    - destruct v as [b v].
+      simpl in *.
+      specialize (IHn m v (word.add addr (word.of_Z 1)) (ptsto addr b * R)%type).
+      rewrite IHn.
+      + erewrite get_sep; [reflexivity|].
+        apply sep_assoc in H.
+        exact H.
+      + apply sep_assoc.
+        (* TODO should "ecancel" do this step as well? *)
+        revert H. clear -mem_ok. revert m.
+        match goal with
+        | |- forall m, ?P m -> ?Q m => change (impl1 P Q)
+        end.
+        (* TODO why does "ecancel" not solve this? *)
+        (* manually: *)
+        apply impl1_sep_cancel_r.
+        intros x H.
+        match type of H with
+        | (?p * ?q)%type x => pose proof (sep_comm p q) as C
+        end.
+        apply C.
+        apply H.
+  Qed.
+
+  Definition ptsto_instr(addr: word)(instr: Instruction): mem -> Prop :=
+    ex1 (fun (w: w32) =>
+           sep (ptsto_bytes 4 addr w)
+               (emp (decode (RV_wXLEN_IM (B := BitWidth)) (LittleEndian.combine 4 w) = instr))).
+
+  Definition program(addr: word)(prog: list Instruction): mem -> Prop :=
+    array ptsto_instr (word.of_Z 4) addr prog.
+
+  Lemma go_fetch_inst: forall {inst initialL pc0} {R: mem -> Prop} (post: RiscvMachineL -> Prop),
       pc0 = initialL.(getPc) ->
-      containsProgram initialL.(getMem) [inst] pc0 ->
+      (program pc0 [inst] * R) initialL.(getMem) ->
       mcomp_sat (Bind (execute inst) (fun _ => step)) initialL post ->
       mcomp_sat (run1 (B := BitWidth)) initialL post.
   Proof.
     intros. subst.
     unfold run1.
     apply go_getPC.
-    unfold containsProgram in H0.
-    specialize (H0 0 _ eq_refl).
-    unfold ldInst in *.
-    destruct_one_match_hyp; [|discriminate].
-    apply invert_Some_eq_Some in H0. subst inst.
-    eapply go_loadWord; [|eassumption].
-    match goal with
-    | H: Memory.loadWord ?m ?pc = ?r |- Memory.loadWord ?m ?pc' = ?r =>
-      replace pc' with pc; [exact H|]
-    end.
-    change (4 * 0) with 0. ring'.
-  Qed.
+    unfold program, array, ptsto_instr in H0.
+    (* TODO how can I destruct this existential? *)
+    eapply go_loadWord.
+    - eapply ptsto_bytes_to_load.
+      (* TODO this is implied by H0 *)
+      admit.
+    - (* TODO this is implied by H1 and the equality "inst = ..." in H0 *)
+      admit.
+  Admitted.
 
 End Go.
