compiler/src/SeparationLogic.v
@@ -1,0 +1,10 @@
+Require Export Coq.Lists.List. Export ListNotations.
+Require Export Coq.ZArith.BinInt. Open Scope Z_scope.
+Require Export coqutil.Word.Interface coqutil.Word.Properties.
+Require Export coqutil.Map.Interface.
+Require Export bedrock2.Lift1Prop.
+Require Export bedrock2.Map.Separation.
+Require Export bedrock2.Map.SeparationLogic.
+Require Export bedrock2.Array.
+
+Infix "*" := sep : type_scope.
